Core/RefinesFacts.v
@@ -906,11 +906,6 @@ easy.
 congruence.
 Qed.
 
-Ltac dec_eq_nats i j :=
-  let H := fresh in
-  assert (H : i = j \/ i <> j) by apply excluded_middle;
-  destruct H; subst.
-
 Inductive Interleave {E F} : (nat -> Trace (LEvent E F)) -> Trace (ThreadLEvent E F) -> Prop :=
 | InterleaveEnd qc :
     (forall i, qc i = nil) ->
@@ -1385,6 +1380,21 @@ assert (forall i, projUnderThrSeq (projPoint i eqb p) = projUnderThrSeq (projPoi
 }
 apply full_projUnderThr_help; easy.
 Qed.
+
+(* Inductive help66_interleave {E F G} : Trace (LEvent E F) -> Trace (LEvent F G) -> Trace (LEvent E G) -> Prop :=
+| HNil :
+    help66_interleave nil nil nil
+| HSkipOverUnder e p q r :
+    help66_interleave p q r ->
+    help66_interleave p (UEvent e :: q) r
+| HSkipUnderOver e p q r :
+    help66_interleave p q r ->
+    help66_interleave (OEvent e :: p) q r
+| HSkipUnderSilent p q r :
+    help66_interleave p q r ->
+    help66_interleave (UEvent None :: p) q r
+| HCons ue oe p q r :
+. *)
 
 Lemma help66 {E F G} (impl : Impl E F) (impl' : Impl F G) sL' sH' :
   forall (tL : list (LEvent E F)) (tH : list (LEvent F G)),
@@ -2034,37 +2044,18 @@ Inductive over_silent_trace {E F} : Trace (LEvent E F) -> Prop :=
 Lemma get_projUnder_over {E F F'} :
   forall q f ev,
   ev :: projUnderThrSeq (F:=F) q = projUnderThrSeq (F:=F') f ->
-  exists u s,
+  (exists n ev' u s,
     over_silent_trace (E:=E) u /\
-    f = u ++ UEvent (Some ev) :: s.
+    f = nones n ++ OEvent ev' :: u ++ UEvent (Some ev) :: s) \/
+  (exists n s,
+    f = nones n ++ UEvent (Some ev) :: s).
 intros.
 generalize dependent q.
 induction f; simpl; intros.
 discriminate.
 destruct a.
 destruct ev0.
-{
-  dependent destruction H.
-  exists nil, f.
-  repeat constructor.
-}
-{
-  apply IHf in H.
-  destruct_all.
-  subst.
-  exists (UEvent None :: x), x0.
-  repeat constructor; try easy.
-  unfold not. intros. destruct_all. discriminate.
-}
-{
-  apply IHf in H.
-  destruct_all.
-  subst.
-  exists (OEvent ev0 :: x), x0.
-  repeat constructor; try easy.
-  unfold not. intros. destruct_all. discriminate.
-}
-Qed.
+Admitted.
 
 Lemma get_projOver_under {E E' F} :
   forall q f ev,
@@ -2459,110 +2450,26 @@ destruct p, q.
   {
     assert (H' := H).
     assert (H0' := H0).
-    specialize (H n).
-    specialize (H0 n0).
-    rewrite eqb_id in *.
-    simpl in *.
-    apply get_projOver_under in H0.
-    destruct H0; destruct_all.
+    specialize (H n). rewrite eqb_id in H. simpl in H.
+    apply get_projUnder_over in H.
+    destruct H; destruct_all.
+    (* there is a blocking overlay event *)
     {
-      assert (H'' := H').
-      specialize (H' n0).
-      rewrite H2, projUnderThrSeq_app, projUnderThrSeq_nones in H'. simpl in *.
-      dec_eq_nats n0 n.
+      specialize (H0 n). rewrite H2, projOverSeq_app, projOverSeq_nones in H0.
+      simpl in *.
+      dec_eq_nats n n0.
       {
-        rewrite eqb_id in *. simpl in *.
-        dependent destruction H'.
-        eassert _.
-        {
-          eapply get_choose_trace with (qc:=fun i => if n =? i then x1 ++ OEvent ev0 :: x2 else qc i) (p:=p) (q:= (n, OEvent ev0) :: q).
-          simpl. lia.
-          intros.
-          dec_eq_nats n i.
-          rewrite eqb_id.
-          easy.
-          rewrite eqb_nid.
-          specialize (H'' i).
-          rewrite eqb_nid in H''.
-          easy.
-          easy.
-          easy.
-          simpl.
-          intros.
-          dec_eq_nats i n.
-          rewrite eqb_id.
-          specialize (H0' n).
-          rewrite eqb_id, H2, projOverSeq_app, projOverSeq_nones in H0'.
-          easy.
-          repeat rewrite eqb_nid.
-          specialize (H0' i).
-          rewrite eqb_nid in H0'.
-          easy.
-          easy.
-          easy.
-          easy.
-          intros.
-          apply H1 in H3.
-          dec_eq_nats i n.
-          rewrite H2 in H3.
-          destruct x0; simpl in H3; discriminate.
-          rewrite eqb_nid.
-          easy.
-          easy.
-        }
-        destruct_all.
-        exists (thread_nones n x0 ++ (n, UEvent (Some x3)) :: x4).
-        clear H'' x H0' H1 get_choose_trace.
-        generalize dependent qc.
-        induction x0; intros.
-        {
-          simpl in *.
-          econstructor.
-          exact H3.
-          easy.
-        }
-        {
-          simpl in *.
-          rewrite H2 in H.
-          simpl in H.
-          rewrite projUnderThrSeq_app, projUnderThrSeq_nones in H.
-          simpl in *.
-          eapply ChooseSilent with (s:= nones x0 ++ UEvent (Some x3) :: _).
-          apply IHx0.
-          rewrite eqb_id.
-          simpl.
-          rewrite projUnderThrSeq_app, projUnderThrSeq_nones.
-          exact H.
-          rewrite eqb_id.
-          easy.
-          rewrite if_prune.
-          easy.
-          easy.
-        }
+        admit.
       }
       {
-        rewrite eqb_nid in *.
-        symmetry in H'.
-        assert (H''' := H'').
-        specialize (H'' n).
-        rewrite eqb_id in H''. simpl in H''.
-        apply get_projUnder_over in H''.
-        destruct H''; destruct_all; subst.
-        2: easy.
-        
+        rewrite eqb_nid in H0.
+        admit.
+        admit.
       }
     }
+    (* there is no blocking overlay event*)
     {
-      eassert _.
-      {
-        eapply get_choose_trace with (p:= (n, UEvent (Some e)) :: p) (q:=q) (qc:=fun i => if n =? i then x0 else qc i).
-        simpl. lia.
-        intros. simpl.
-        specialize (H' i).
-        dec_eq_nats i n.
-        rewrite eqb_id in *. simpl in *.
-        
-      }
+      admit.
     }
   }
   {
@@ -2647,15 +2554,10 @@ assert (
     choose_trace qc p q r
 ).
 {
-  rewrite fmap_correct with (qc:=qc) (is:= map fst p ++ map fst q).
-  apply get_choose_trace.
-  rewrite <- fmap_correct.
+  eapply get_choose_trace.
   easy.
   easy.
-  rewrite <- fmap_correct.
-  easy.
-  easy.
-  easy.
+  exact H1.
 }
 destruct_all.
 exists x.
